Progress on new chacha20

code/salsa-family/Hacl.Impl.Chacha20.fst
@@ -223,7 +223,7 @@ let double_round st =
 
 
 [@ "c_inline"]
-val rounds: st:state ->
+assume val rounds: st:state ->
   Stack unit
     (requires (fun h -> live h st))
     (ensures  (fun h0 _ h1 -> preserves_live h0 h1 /\ modifies1 st h0 h1))
@@ -265,7 +265,7 @@ let sum_states st st' = map2 (fun x y -> x +. y) st st'
 
 
 [@ "c_inline"]
-val copy_state:
+assume val copy_state:
   st:state ->
   st':state ->
   Stack unit
@@ -283,13 +283,14 @@ let spec_f = Spec.iteri n ()
   // Seq.lemma_eq_intro (as_seq h st) (Seq.slice (as_seq h st) 0 16);
   // Seq.lemma_eq_intro (as_seq h st') (Seq.slice (as_seq h st') 0 16);
   // Seq.lemma_eq_intro (as_seq h st) (as_seq h st')
-
+*)
 
 #reset-options " --max_fuel 0 --z3rlimit 100"
 
-type log_t_ = | MkLog: k:Spec.key -> n:Spec.nonce -> log_t_
+noeq type log_t_ = | MkLog: k:Spec.key -> n:Spec.nonce -> log_t_
 type log_t = Ghost.erased log_t_
 
+(*
 private
 val lemma_setup_inj:
   k:Spec.key -> n:Spec.nonce -> c:Spec.counter ->
@@ -345,7 +346,7 @@ val lemma_state_counter:
   k:Spec.key -> n:Spec.nonce -> c:Spec.counter ->
   Lemma (U32.v (Seq.index (Spec.setup k n (c)) 12) == c)
 let lemma_state_counter k n c = ()
-
+*)
 
 #reset-options "--max_fuel 0  --z3rlimit 400"
 
@@ -354,69 +355,74 @@ private
 val chacha20_core:
   log:log_t ->
   k:state ->
-  st:state{disjoint st k} ->
-  ctr:UInt32.t ->
+  st:state ->
+  ctr:size_t ->
   Stack log_t
-    (requires (fun h -> live h k /\ live h st /\ invariant log h st))
-    (ensures  (fun h0 updated_log h1 -> live h0 st /\ live h0 k /\ invariant log h0 st
-      /\ live h1 k /\ invariant updated_log h1 st /\ modifies_2 k st h0 h1
-      /\ (let key = reveal_h32s (as_seq h1 k) in
-          let stv = reveal_h32s (as_seq h1 st) in
-          Seq.index stv 12 == ctr /\
-         (match Ghost.reveal log, Ghost.reveal updated_log with
-         | MkLog k n, MkLog k' n' ->
-             key == chacha20_core stv /\ k == k' /\ n == n'))))
+    (requires (fun h -> live h k /\ live h st /\ disjoint st k)) // /\ invariant log h st))
+    (ensures  (fun h0 updated_log h1 -> preserves_live h0 h1 /\ modifies2 st k h0 h1))
+      // live h0 st /\ live h0 k /\ invariant log h0 st
+      // /\ live h1 k /\ invariant updated_log h1 st /\ modifies_2 k st h0 h1
+      // /\ (let key = reveal_h32s (as_seq h1 k) in
+      //     let stv = reveal_h32s (as_seq h1 st) in
+      //     Seq.index stv 12 == ctr /\
+      //    (match Ghost.reveal log, Ghost.reveal updated_log with
+      //    | MkLog k n, MkLog k' n' ->
+      //        key == chacha20_core stv /\ k == k' /\ n == n'))))
 [@ "c_inline"]
 let chacha20_core log k st ctr =
-  let h_0 = ST.get() in
-  st.(12ul) <- uint32_to_sint32 ctr;
-  lemma_invariant (reveal_h32s (as_seq h_0 st)) (Ghost.reveal log).k (Ghost.reveal log).n (get h_0 st 12) (uint32_to_sint32 ctr);
+  (**) let h0 = ST.get() in
+  st.(12) <- u32 ctr;
+  (**) let h1 = ST.get () in
+  (**) assume(disjoint k st);
   copy_state k st;
-  let h' = ST.get() in
-  cut (as_seq h' k == as_seq h' st);
+  (**) let h2 = ST.get () in
   rounds k;
-  let h'' = ST.get() in
-  cut (reveal_h32s (as_seq h'' k) == Spec.Chacha20.rounds (reveal_h32s (as_seq h' st)));
+  (**) let h3 = ST.get () in
   sum_states k st;
-  let h = ST.get() in
-  cut (reveal_h32s (as_seq h k) == chacha20_core (reveal_h32s (as_seq h st)));
+  (**) let h4 = ST.get () in
+  (**) assume(modifies1 st h0 h1 /\ modifies1 k h1 h2 /\ modifies1 k h2 h3 /\ modifies1 k h3 h4 ==> modifies2 st k h0 h4);
   Ghost.elift1 (fun l -> match l with | MkLog k n -> MkLog k n) log
 
 
 [@ "c_inline"]
 val chacha20_block:
   log:log_t ->
-  stream_block:uint8_p{length stream_block = 64} ->
-  st:state{disjoint st stream_block} ->
-  ctr:UInt32.t ->
+  stream_block:lbuffer uint8 64 ->
+  st:state ->
+  ctr:size_t ->
   Stack log_t
-    (requires (fun h -> live h stream_block /\ invariant log h st))
-    (ensures  (fun h0 updated_log h1 -> live h1 stream_block /\ invariant log h0 st
-      /\ invariant updated_log h1 st /\ modifies_2 stream_block st h0 h1
-      /\ (let block = reveal_sbytes (as_seq h1 stream_block) in
-         match Ghost.reveal log, Ghost.reveal updated_log with
-         | MkLog k n, MkLog k' n' ->
-             block == chacha20_block k n (U32.v ctr) /\ k == k' /\ n == n')))
+    (requires (fun h -> live h stream_block /\ live h st /\ disjoint stream_block st))///\ invariant log h st))
+    (ensures  (fun h0 updated_log h1 -> preserves_live h0 h1 /\ modifies2 stream_block st h0 h1))
+      // live h1 stream_block /\ invariant log h0 st
+      // /\ invariant updated_log h1 st /\ modifies_2 stream_block st h0 h1
+      // /\ (let block = reveal_sbytes (as_seq h1 stream_block) in
+      //    match Ghost.reveal log, Ghost.reveal updated_log with
+      //    | MkLog k n, MkLog k' n' ->
+      //        block == chacha20_block k n (U32.v ctr) /\ k == k' /\ n == n')))
 [@ "c_inline"]
 let chacha20_block log stream_block st ctr =
-  (**) let hinit = ST.get() in
-  push_frame();
-  (**) let h0 = ST.get() in
-  (**) let h_0 = ST.get() in
-  let st' = Buffer.create (uint32_to_sint32 0ul) 16ul in
-  (**) let h1 = ST.get() in
+  (**) let h0 = ST.get () in
+  (**) push_frame();
+  (**) let h1 = ST.get () in
+  // BB. Fix this temporary bypass
+  (**) assume(modifies0 h0 h1);
+  let st' = create 16 (u32 0) in
+  (**) let h2 = ST.get () in
+  (**) assume(disjoint st st');
+  (**) assume(live h2 st);
   let log' = chacha20_core log st' st ctr in
-  (**) let h2 = ST.get() in
-  (**) lemma_modifies_0_2' st st' h0 h1 h2;
-  uint32s_to_le_bytes stream_block st' 16ul;
-  (**) let h = ST.get() in
-  (**) lemma_modifies_2_1'' st stream_block h0 h2 h;
-  (**) assert (reveal_sbytes (as_seq h stream_block) == chacha20_block (Ghost.reveal log').k (Ghost.reveal log').n (U32.v ctr));
-  (**) assert (modifies_3_2 stream_block st h_0 h);
-  pop_frame();
-  (**) let hfin = ST.get() in
-  (**) modifies_popped_3_2 stream_block st hinit h0 h hfin;
+  (**) let h3 = ST.get () in
+  (**) assume(live h3 stream_block);
+  (**) assume(disjoint stream_block st');
+  uint32s_to_bytes_le 16 stream_block st';
+  (**) let h4 = ST.get () in
+  (**) pop_frame();
+  (**) let h5 = ST.get () in
+  // BB. Fix this temporary bypass
+  (**) assume(modifies0 h4 h5);
+  (**) assume(modifies0 h0 h1 /\ modifies1 st' h1 h2 /\ modifies2 st st' h2 h3 /\ modifies1 stream_block h3 h4 /\ modifies0 h4 h5 ==> modifies2 stream_block st h0 h5);
   (**) Ghost.elift1 (fun l -> match l with | MkLog k n -> MkLog k n) log'
+
 
 
 [@ "c_inline"]
@@ -424,31 +430,33 @@ val alloc:
   unit ->
   StackInline state
     (requires (fun h -> True))
-    (ensures (fun h0 st h1 -> (st `unused_in` h0) /\ live h1 st /\ modifies_0 h0 h1 /\ frameOf st == h1.tip
-      /\ Map.domain h1.h == Map.domain h0.h))
+    (ensures (fun h0 st h1 -> True))
+                           // (st `unused_in` h0) /\ live h1 st /\ modifies0 h0 h1 /\ 
+                           // frameOf st == h1.tip /\ Map.domain h1.h == Map.domain h0.h))
 [@ "c_inline"]
-let alloc () =
-  create (uint32_to_sint32 0ul) 16ul
+let alloc () = create 16 (u32 0)
 
 
 [@ "c_inline"]
 val init:
   st:state ->
-  k:uint8_p{length k = 32 /\ disjoint st k} ->
-  n:uint8_p{length n = 12 /\ disjoint st n} ->
+  k:lbuffer uint8 32 ->
+  n:lbuffer uint8 12 ->
   Stack log_t
-    (requires (fun h -> live h k /\ live h n /\ live h st))
-    (ensures  (fun h0 log h1 -> live h1 st /\ live h0 k /\ live h0 n /\ modifies_1 st h0 h1
-      /\ invariant log h1 st
-      /\ (match Ghost.reveal log with MkLog k' n' -> k' == reveal_sbytes (as_seq h0 k)
-           /\ n' == reveal_sbytes (as_seq h0 n))))
+    (requires (fun h -> live h k /\ live h n /\ live h st /\ disjoint st k /\ disjoint st n /\ disjoint k n))
+    (ensures  (fun h0 log h1 -> preserves_live h0 h1 /\ modifies1 st h0 h1))
+      // /\ invariant log h1 st
+      // /\ (match Ghost.reveal log with MkLog k' n' -> k' == reveal_sbytes (as_seq h0 k)
+      //      /\ n' == reveal_sbytes (as_seq h0 n))))
+
 [@ "c_inline"]
 let init st k n =
-  setup st k n 0ul;
+  setup st k n 0;
   let h = ST.get() in
-  Ghost.elift2 (fun (k:uint8_p{length k = 32 /\ live h k}) (n:uint8_p{length n = 12 /\ live h n}) -> MkLog (reveal_sbytes (as_seq h k)) (reveal_sbytes (as_seq h n))) (Ghost.hide k) (Ghost.hide n)
+  Ghost.elift2 (fun (k:lbuffer uint8 32) (n:lbuffer uint8 12) -> MkLog (as_lseq k h) (as_lseq n h)) (Ghost.hide k) (Ghost.hide n)
 
 
+(*
 #reset-options " --max_fuel 0 --z3rlimit 100"
 
 val lemma_chacha20_counter_mode_1:
@@ -519,94 +527,109 @@ val lemma_chacha20_counter_mode_0:
 #reset-options "--initial_fuel 1 --max_fuel 1 --z3rlimit 100"
 let lemma_chacha20_counter_mode_0 ho output hi input len k n ctr =
   Seq.lemma_eq_intro (as_seq ho output) Seq.createEmpty
-
+*)
 
 #reset-options " --max_fuel 0 --z3rlimit 400"
 
 val update_last:
-  output:uint8_p ->
-  plain:uint8_p{disjoint output plain} ->
-  len:U32.t{U32.v len = length output /\ U32.v len = length plain /\ U32.v len < 64 /\ UInt32.v len > 0} ->
+  len:size_t{0 < len /\ len < 64} ->
+  output:lbuffer uint8 len ->
+  plain:lbuffer uint8 len ->
   log:log_t ->
-  st:state{disjoint st output /\ disjoint st plain} ->
-  ctr:UInt32.t{UInt32.v ctr + (length plain / 64) < pow2 32} ->
+  st:state ->
+  ctr:size_t{ctr + (len / 64) <= max_size_t} ->
   Stack log_t
-    (requires (fun h -> live h output /\ live h plain /\ invariant log h st))
-    (ensures (fun h0 updated_log h1 -> live h1 output /\ live h0 plain /\ invariant updated_log h1 st
-      /\ modifies_2 output st h0 h1
-      /\ (let o = reveal_sbytes (as_seq h1 output) in
-         let plain = reveal_sbytes (as_seq h0 plain) in
-         match Ghost.reveal log with | MkLog k n ->
-         o == (let mask = chacha20_cipher k n (UInt32.v ctr+(UInt32.v len / 64)) in
-               let mask = Seq.slice mask 0 (UInt32.v len) in
-               Spec.CTR.xor #(UInt32.v len) plain mask))))
-let update_last output plain len log st ctr =
+    (requires (fun h -> live h output /\ live h plain /\ disjoint output plain /\ disjoint st output /\ disjoint st plain)) //invariant log h st))
+    (ensures (fun h0 updated_log h1 -> preserves_live h0 h1 /\ modifies2 output st h0 h1))
+      // live h1 output /\ live h0 plain /\ invariant updated_log h1 st
+      // /\ (let o = reveal_sbytes (as_seq h1 output) in
+      //    let plain = reveal_sbytes (as_seq h0 plain) in
+      //    match Ghost.reveal log with | MkLog k n ->
+      //    o == (let mask = chacha20_cipher k n (UInt32.v ctr+(UInt32.v len / 64)) in
+      //          let mask = Seq.slice mask 0 (UInt32.v len) in
+      //          Spec.CTR.xor #(UInt32.v len) plain mask))))
+
+let update_last len output plain log st ctr =
   (**) let h0 = ST.get() in
   push_frame();
-  (**) let h = ST.get() in
-  let block = create (uint8_to_sint8 0uy) 64ul in
-  (**) let h' = ST.get() in
-  let l = chacha20_block log block st ctr in
-  (**) let h'' = ST.get() in
-  (**) lemma_modifies_0_2' st block h h' h'';
-  let mask = Buffer.sub block 0ul len in
-  map2 output plain mask len (fun x y -> H8.(x ^^ y));
   (**) let h1 = ST.get() in
-  (**) lemma_modifies_2_1'' st output h h'' h1;
-  (**) lemma_chacha20_counter_mode_1 h1 output h0 plain len (Ghost.reveal log).k (Ghost.reveal log).n ctr;
+  // BB. Fix this temporary bypass
+  assume(modifies0 h0 h1);
+  let block = create 64 (u8 0) in
+  (**) let h2 = ST.get() in
+  (**) assume(disjoint block st);
+  (**) assume(live h2 st);
+  (**) assume(disjoint block plain);
+  (**) assume(live h2 plain);
+  (**) assume(disjoint block output);
+  (**) assume(live h2 output);
+  let l = chacha20_block log block st ctr in
+  (**) let h3 = ST.get() in
+  let mask = sub block 0 len in
+  (**) let h4 = ST.get () in
+  // BB. This is highly unlikely to work !
+  // map2 has to be changed
+  map2 (fun x y -> x ^. y) output plain;
+  map2 (fun x y -> x ^. y) output mask;
+  (**) let h5 = ST.get() in
   pop_frame();
-  (**) let hfin = ST.get() in
-  (**) modifies_popped_3_2 st output h0 h h1 hfin;
+  (**) let h6 = ST.get() in
+  (**) assume(modifies0 h5 h6);
+  (**) assume (modifies0 h0 h1 /\ modifies1 block h1 h2 /\ modifies2 block st h2 h3 /\ modifies0 h3 h4 /\ modifies1 output h4 h5 /\ modifies0 h5 h6 ==> modifies2 output st h0 h6);
   l
 
 
 val update:
-  output:uint8_p{length output = 64} ->
-  plain:uint8_p{disjoint output plain /\ length plain = 64} ->
+  output:lbuffer uint8 64 ->
+  plain:lbuffer uint8 64->
   log:log_t ->
-  st:state{disjoint st output /\ disjoint st plain} ->
-  ctr:U32.t{U32.v ctr + 1 < pow2 32} ->
+  st:state ->
+  ctr:size_t{ctr + 1 <= max_size_t} ->
   Stack log_t
-    (requires (fun h -> live h output /\ live h plain /\ invariant log h st))
-    (ensures (fun h0 updated_log h1 -> live h1 output /\ live h0 plain /\ invariant updated_log h1 st
-      /\ modifies_2 output st h0 h1
-      /\ updated_log == log
-      /\ (let o = reveal_sbytes (as_seq h1 output) in
-         let plain = reveal_sbytes (as_seq h0 plain) in
-         match Ghost.reveal log with | MkLog k n ->
-         o == seq_map2 (fun x y -> FStar.UInt8.(x ^^ y)) plain (chacha20_cipher k n (U32.v ctr)))))
+    (requires (fun h -> live h output /\ live h plain /\ disjoint st output /\ disjoint st plain)) //invariant log h st))
+    (ensures (fun h0 updated_log h1 -> live h1 output /\ live h0 plain /\ modifies2 output st h0 h1))
+      // /\ invariant updated_log h1 st
+      // /\ modifies_2 output st h0 h1
+      // /\ updated_log == log
+      // /\ (let o = reveal_sbytes (as_seq h1 output) in
+      //    let plain = reveal_sbytes (as_seq h0 plain) in
+      //    match Ghost.reveal log with | MkLog k n ->
+      //    o == seq_map2 (fun x y -> FStar.UInt8.(x ^^ y)) plain (chacha20_cipher k n (U32.v ctr)))))
+
 let update output plain log st ctr =
-  let h0 = ST.get() in
+  (**) let h0 = ST.get() in
   push_frame();
   (**) let h1 = ST.get() in
-  let b  = create (uint32_to_sint32 0ul) 48ul in
+  let b  = create 48 (u32 0) in
   (**) let h2 = ST.get() in
-  let k  = Buffer.sub b 0ul  16ul in
-  let ib = Buffer.sub b 16ul 16ul in
-  let ob = Buffer.sub b 32ul 16ul in
+  let k  = sub b 0  16 in
+  let ib = sub b 16 16 in
+  let ob = sub b 32 16 in
   let l  = chacha20_core log k st ctr in
   (**) let h3 = ST.get() in
-  (**) modifies_subbuffer_2 h2 h3 k st b;
-  uint32s_from_le_bytes ib plain 16ul;
+  // (**) modifies_subbuffer_2 h2 h3 k st b;
+  uint32s_from_bytes_le 16 ib plain;
   (**) let h  = ST.get() in
-  (**) modifies_subbuffer_1 h3 h ib b;
-  map2 ob ib k 16ul (fun x y -> H32.(x ^^ y));
+  // (**) modifies_subbuffer_1 h3 h ib b;
+  map2 (fun x y -> x ^. y) ob ib;
+  map2 (fun x y -> x ^. y) ob k;
+  // map2 ob ib k 16 (fun x y -> x ^. y);
   (**) let h4  = ST.get() in
-  (**) modifies_subbuffer_1 h h4 ob b;
-  (**) lemma_modifies_1_trans b h3 h h4;
-  (**) lemma_modifies_2_1' b st h2 h3 h4;
-  (**) lemma_modifies_0_2 st b h1 h2 h4;
-  uint32s_to_le_bytes output ob 16ul;
+  // (**) modifies_subbuffer_1 h h4 ob b;
+  // (**) lemma_modifies_1_trans b h3 h h4;
+  // (**) lemma_modifies_2_1' b st h2 h3 h4;
+  // (**) lemma_modifies_0_2 st b h1 h2 h4;
+  uint32s_to_bytes_le 16 output ob;
   (**) let h5  = ST.get() in
-  (**) lemma_modifies_2_1'' st output h1 h4 h5;
-  Hacl.Impl.Xor.Lemmas.lemma_xor_uint32s_to_bytes (reveal_sbytes (as_seq h0 plain))
-                                                       (reveal_h32s (as_seq h k));
+  // (**) lemma_modifies_2_1'' st output h1 h4 h5;
+  // Hacl.Impl.Xor.Lemmas.lemma_xor_uint32s_to_bytes (reveal_sbytes (as_seq h0 plain))
+  //                                                      (reveal_h32s (as_seq h k));
   pop_frame();
-  (**) let hfin = ST.get() in
-  (**) modifies_popped_3_2 st output h0 h1 h5 hfin;
+  (**) let h6 = ST.get() in
+  // (**) modifies_popped_3_2 st output h0 h1 h5 hfin;
   l
 
-
+(*
 #reset-options " --max_fuel 0 --z3rlimit 100"
 
 private
@@ -627,84 +650,88 @@ val lemma_chacha20_counter_mode_def_0:
 let lemma_chacha20_counter_mode_def_0 s k n ctr =
   Seq.lemma_eq_intro s Seq.createEmpty
 
-
+*)
 #reset-options "--max_fuel 0  --z3rlimit 200"
 
 private
 val chacha20_counter_mode_blocks:
-  output:uint8_p ->
-  plain:uint8_p{disjoint output plain} ->
-  len:UInt32.t{64 * UInt32.v len = length output /\ length output = length plain} ->
+  len:size_t ->
+  output:lbuffer uint8 len ->
+  plain:lbuffer uint8 len ->
   log:log_t ->
-  st:state{disjoint st output /\ disjoint st plain} ->
-  ctr:UInt32.t{UInt32.v ctr + (length plain / 64) < pow2 32} ->
+  st:state ->
+  ctr:size_t{ctr + (len / 64) <= max_size_t} ->
   Stack unit
-    (requires (fun h -> live h output /\ live h plain /\ invariant log h st))
-    (ensures (fun h0 _ h1 -> live h1 output /\ live h0 plain /\ live h1 st
-      /\ modifies_2 output st h0 h1 /\ invariant log h1 st
-      /\ (let o = reveal_sbytes (as_seq h1 output) in
-         let plain = reveal_sbytes (as_seq h0 plain) in
-         match Ghost.reveal log with | MkLog k n ->
-         o == Spec.CTR.counter_mode_blocks chacha20_ctx chacha20_cipher k n (UInt32.v ctr) plain)))
+    (requires (fun h -> live h output /\ live h plain
+              /\ disjoint output plain /\ disjoint st output /\ disjoint st plain)) ///\ invariant log h st))
+    (ensures (fun h0 _ h1 -> preserves_live h0 h1 /\ modifies2 output st h0 h1))
+      // live h1 output /\ live h0 plain /\ live h1 st
+      // /\ modifies_2 output st h0 h1 /\ invariant log h1 st
+      // /\ (let o = reveal_sbytes (as_seq h1 output) in
+      //    let plain = reveal_sbytes (as_seq h0 plain) in
+      //    match Ghost.reveal log with | MkLog k n ->
+      //    o == Spec.CTR.counter_mode_blocks chacha20_ctx chacha20_cipher k n (UInt32.v ctr) plain)))
 #reset-options "--max_fuel 0 --z3rlimit 200"
 let chacha20_counter_mode_blocks output plain len log st ctr =
   let h0 = ST.get() in
-  let inv (h1: mem) (i: nat): Type0 =
-    live h1 output /\ invariant log h1 st /\ modifies_2 output st h0 h1 /\ 0 <= i /\ i <= UInt32.v len
-    /\ (match Ghost.reveal log with | MkLog k n ->
-      reveal_sbytes (Seq.slice (as_seq h1 output) 0 (64 * i))
-      == Spec.CTR.counter_mode_blocks chacha20_ctx chacha20_cipher k n (UInt32.v ctr) (reveal_sbytes (Seq.slice (as_seq h0 plain) 0 (64 * i))))
-  in
-  let f' (i:UInt32.t{ FStar.UInt32.( 0 <= v i /\ v i < v len ) }): Stack unit
-    (requires (fun h -> inv h (UInt32.v i)))
-    (ensures (fun h_1 _ h_2 -> FStar.UInt32.(inv h_2 (v i + 1))))
-  = let h = ST.get() in
-    let open FStar.UInt32 in
-    let o'' = Buffer.sub output 0ul (64ul *^ i +^ 64ul) in
-    let b'' = Buffer.sub plain  0ul (64ul *^ i +^ 64ul) in
-    let b  = Buffer.sub plain (64ul *^ i) 64ul in
-    let b' = Buffer.sub plain 0ul (64ul *^ i)  in
-    let o  = Buffer.sub output (64ul *^ i) 64ul in
-    let o' = Buffer.sub output 0ul (64ul *^ i)  in
-    let log' = update o b log st FStar.UInt32.(ctr+^ i) in
-    let h' = ST.get() in
-    (**) modifies_subbuffer_2 h h' o st output;
-    (**) lemma_modifies_2_trans output st h0 h h';
-    no_upd_lemma_2 h h' o st b;
-    no_upd_lemma_2 h h' o st b';
-    no_upd_lemma_2 h h' o st o';
-    Seq.lemma_eq_intro (Seq.slice (as_seq h' output) 0 (64 * v i + 64))
-                       (as_seq h' (Buffer.sub output 0ul (64ul *^ i +^ 64ul)));
-    Seq.lemma_eq_intro (Seq.slice (as_seq h0 plain) 0 (64 * v i + 64))
-                       (as_seq h0 (Buffer.sub plain 0ul (64ul *^ i +^ 64ul)));
-    Seq.lemma_eq_intro (Seq.slice (as_seq h' output) 0 (64 * v i))
-                       (Seq.slice (Seq.slice (as_seq h' output) 0 (64 * v i + 64)) 0 (64 * v i));
-    Seq.lemma_eq_intro (Seq.slice (as_seq h' output) (64 * v i) (64 * v i + 64))
-                       (Seq.slice (Seq.slice (as_seq h' output) 0 (64 * v i + 64)) (64 * v i) (64 * v i + 64));
-    Seq.lemma_eq_intro (Seq.slice (as_seq h0 plain) 0 (64 * v i))
-                       (Seq.slice (Seq.slice (as_seq h0 plain) 0 (64 * v i + 64)) 0 (64 * v i));
-    Seq.lemma_eq_intro (Seq.slice (as_seq h0 plain) (64 * v i) (64 * v i + 64))
-                       (Seq.slice (Seq.slice (as_seq h0 plain) 0 (64 * v i + 64)) (64 * v i) (64 * v i + 64));
-    Seq.lemma_eq_intro (Seq.slice (as_seq h0 plain) 0 (64 * v i + 64))
-                       (Seq.append (Seq.slice (as_seq h0 plain) 0 (64 * v i)) (Seq.slice (as_seq h0 plain) (64 * v i) (64 * v i + 64)));
-    Seq.lemma_eq_intro (Seq.slice (as_seq h' output) 0 (64 * v i + 64))
-                       (Seq.append (Seq.slice (as_seq h' output) 0 (64 * v i)) (Seq.slice (as_seq h' output) (64 * v i) (64 * v i + 64)));
-    lemma_chacha20_counter_mode_2 h o'' h0 b'' (64ul *^ i +^ 64ul) (MkLog?.k (Ghost.reveal log)) (MkLog?.n (Ghost.reveal log)) ctr
-  in
-  let o0 = Buffer.sub output 0ul 0ul in
-  let i0 = Buffer.sub plain  0ul 0ul in
-  Seq.lemma_eq_intro (as_seq h0 o0) (Seq.slice (as_seq h0 output) 0 0);
-  Seq.lemma_eq_intro (as_seq h0 i0) (Seq.slice (as_seq h0 plain) 0 0);
-  lemma_aux_modifies_2 h0 output st;
-  lemma_chacha20_counter_mode_def_0 (Seq.slice (as_seq h0 plain) 0 0) (Ghost.reveal log).k (Ghost.reveal log).n ctr;
-  Seq.lemma_eq_intro (Seq.slice (as_seq h0 plain) 0 0) Seq.createEmpty;
-  Seq.lemma_eq_intro (Seq.slice (as_seq h0 output) 0 0) Seq.createEmpty;
-  C.Loops.for 0ul len inv f';
-  let h = ST.get() in
-  Seq.lemma_eq_intro (Seq.slice (as_seq h output) 0 (64 * UInt32.v len)) (as_seq h output);
-  Seq.lemma_eq_intro (Seq.slice (as_seq h0 plain) 0 (64 * UInt32.v len)) (as_seq h plain)
+  let inv (h1: mem) (i: nat): Type0 = preserves_live h0 h1 /\ modifies2 output st h0 h1 /\ 0 <= i /\ i <= len in
+  //   live h1 output /\ invariant log h1 st /\ modifies_2 output st h0 h1 /\ 0 <= i /\ i <= UInt32.v len
+  //   /\ (match Ghost.reveal log with | MkLog k n ->
+  //     reveal_sbytes (Seq.slice (as_seq h1 output) 0 (64 * i))
+  //     == Spec.CTR.counter_mode_blocks chacha20_ctx chacha20_cipher k n (UInt32.v ctr) (reveal_sbytes (Seq.slice (as_seq h0 plain) 0 (64 * i))))
+  // in
+  let f' (i:size_t{0 <= i /\ i < len}): Stack unit
+    (requires (fun h -> inv h i))
+    (ensures (fun h1 _ h2 -> inv h2 (i + 1)))
+  =
+    // let h = ST.get() in
+    // let open FStar.UInt32 in
+    let o'' = sub output 0 (64 * i + 64) in
+    let b'' = sub plain  0 (64 * i + 64) in
+    let b  = sub plain (64 * i) 64 in
+    let b' = sub plain 0 (64 * i)  in
+    let o  = sub output (64 * i) 64 in
+    let o' = sub output 0 (64 * i)  in
+    let log' = update o b log st (ctr + i) in
+    // let h' = ST.get() in
+    // (**) modifies_subbuffer_2 h h' o st output;
+    // (**) lemma_modifies_2_trans output st h0 h h';
+    // no_upd_lemma_2 h h' o st b;
+    // no_upd_lemma_2 h h' o st b';
+    // no_upd_lemma_2 h h' o st o';
+    // Seq.lemma_eq_intro (Seq.slice (as_seq h' output) 0 (64 * v i + 64))
+    //                    (as_seq h' (Buffer.sub output 0ul (64ul *^ i +^ 64ul)));
+    // Seq.lemma_eq_intro (Seq.slice (as_seq h0 plain) 0 (64 * v i + 64))
+    //                    (as_seq h0 (Buffer.sub plain 0ul (64ul *^ i +^ 64ul)));
+    // Seq.lemma_eq_intro (Seq.slice (as_seq h' output) 0 (64 * v i))
+    //                    (Seq.slice (Seq.slice (as_seq h' output) 0 (64 * v i + 64)) 0 (64 * v i));
+    // Seq.lemma_eq_intro (Seq.slice (as_seq h' output) (64 * v i) (64 * v i + 64))
+    //                    (Seq.slice (Seq.slice (as_seq h' output) 0 (64 * v i + 64)) (64 * v i) (64 * v i + 64));
+    // Seq.lemma_eq_intro (Seq.slice (as_seq h0 plain) 0 (64 * v i))
+    //                    (Seq.slice (Seq.slice (as_seq h0 plain) 0 (64 * v i + 64)) 0 (64 * v i));
+    // Seq.lemma_eq_intro (Seq.slice (as_seq h0 plain) (64 * v i) (64 * v i + 64))
+    //                    (Seq.slice (Seq.slice (as_seq h0 plain) 0 (64 * v i + 64)) (64 * v i) (64 * v i + 64));
+    // Seq.lemma_eq_intro (Seq.slice (as_seq h0 plain) 0 (64 * v i + 64))
+    //                    (Seq.append (Seq.slice (as_seq h0 plain) 0 (64 * v i)) (Seq.slice (as_seq h0 plain) (64 * v i) (64 * v i + 64)));
+    // Seq.lemma_eq_intro (Seq.slice (as_seq h' output) 0 (64 * v i + 64))
+    //                    (Seq.append (Seq.slice (as_seq h' output) 0 (64 * v i)) (Seq.slice (as_seq h' output) (64 * v i) (64 * v i + 64)));
+    // lemma_chacha20_counter_mode_2 h o'' h0 b'' (64ul *^ i +^ 64ul) (MkLog?.k (Ghost.reveal log)) (MkLog?.n (Ghost.reveal log)) ctr
+  // in
+  let o0 = sub output 0 0 in
+  let i0 = sub plain  0 0 in
+  // Seq.lemma_eq_intro (as_seq h0 o0) (Seq.slice (as_seq h0 output) 0 0);
+  // Seq.lemma_eq_intro (as_seq h0 i0) (Seq.slice (as_seq h0 plain) 0 0);
+  // lemma_aux_modifies_2 h0 output st;
+  // lemma_chacha20_counter_mode_def_0 (Seq.slice (as_seq h0 plain) 0 0) (Ghost.reveal log).k (Ghost.reveal log).n ctr;
+  // Seq.lemma_eq_intro (Seq.slice (as_seq h0 plain) 0 0) Seq.createEmpty;
+  // Seq.lemma_eq_intro (Seq.slice (as_seq h0 output) 0 0) Seq.createEmpty;
+  repeati 0 len inv f';
+  // let h = ST.get() in
+  // Seq.lemma_eq_intro (Seq.slice (as_seq h output) 0 (64 * UInt32.v len)) (as_seq h output);
+  // Seq.lemma_eq_intro (Seq.slice (as_seq h0 plain) 0 (64 * UInt32.v len)) (as_seq h plain)
+  ()
 
-
+(*
 val chacha20_counter_mode:
   output:uint8_p ->
   plain:uint8_p{disjoint output plain} ->
